



$L(a) = \{a\}$	(singleton set) for every character $a \in \Sigma$
$L(0) = \{\}$	(the empty language, no strings)
$L(1) = \{\epsilon\}$	(the language consisting of the empty string)
$L(r_1 + r_2) = \{s   s \in L(r_1) \text{ or } s \in L(r_2)\}$	
$L(r_1 r_2) = \{s_1 s_2   s_1 \in L(r_1) \text{ and } s_2 \in L(r_2)\}$	
$L(r^*) = \{s   s = s_1 s_2 \dots s_n, \text{ some } n \geq 0, \text{ with each } s_i \in L(r)\}$	

$\{\epsilon, "a", "b", "ab"\}$	$(a+1)(b+1)$
set of all strings with no consecutive "b"	$(a+ba)^*(b+1)$

```

fun rev (Times (r1, r2)) = Times (rev r2, rev r1)
  | rev (Plus (r1, r2)) = Plus (rev r1, rev r2)
  | rev (Star r) = Star (rev r)

fun ap (Char c) = Plus (One, Char c) (* all prefixes *)
  | ap (Times (r1, r2)) = Plus (ap r1, Times (r1, ap r2))
  | ap (Plus (r1, r2)) = Plus (ap r1, ap r2)
  | ap (Star r) = Times (Star r, ap r)

fun nub One = Zero (* remove One *)
  | nub Plus (r1,r2) = Plus (nub r1, nub r2)
  | nub Times (r1,r2) =
    Plus (Times (nub r1, r2), Times (r1,nub r2))
  | nub Star r = Times (nub r, Star r)

fun match (r : regexp) (cs : char list)
  (k : char list -> bool) : bool = case r of
  Zero    => false
  | One    => k cs
  | Char c => (case cs of [] => false
    | c' :: cs' => c' = c andalso k cs')
  | Plus (r1,r2) => match r1 cs k orelse match r2 cs k
  | Times (r1,r2) => match r1 cs (fn cs' => match r2 cs' k)
  | Star r =>
    k cs orelse match r cs (fn cs' => match (Star r) cs' k)
  | Star r =>
    let fun m' cs' = k cs' orelse match r cs' m' in m' cs end
    fun accept r s = match r (String.explode s) List.null

```

```

fun flatten ([] : int list list) : int list = []
  | flatten (L :: LS) = (case L of
    [] => flatten LS
    | x :: xs => x :: (flatten (xs :: LS)))

```

We want to show that for all values  $LL : \text{int list list}$ ,  $\text{flatten } LL \cong \text{oldFlat } LL$ .

**Proof:** We proceed by structural induction on  $LL$

**Base Case:**  $LL = []$  ... Hence,  $\text{flatten } [] \cong \text{oldFlat } []$

**Inductive Case:**  $LL = L :: LS$  for some values  $L : \text{int list}$  and  $LS : \text{int list list}$

**Inductive Hypothesis:** Assume  $\text{flatten } LS \cong \text{oldFlat } LS$

**Want to show:**  $\text{flatten } L :: LS \cong \text{oldFlat } L :: LS$

We then proceed by structural induction on  $L$

Inner Base Case: Let  $L \cong []$  ...

Inner Inductive Case: Let  $L \cong x :: xs$  for some  $x : \text{int}$  and  $xs : \text{int list}$

Inner IH:  $\text{flatten } (xs :: LS) \cong \text{oldFlat } (xs :: LS)$

WTS:  $\text{flatten } ((x::xs)::LS) \cong \text{oldFlat } ((x::xs)::LS)$

[cite outer/inner IH, **totality**, clause # of function]

Since  $\text{flatten } L :: LS \cong \text{oldFlat } L :: LS$ , by structural induction on  $LL$ , for all  $LL : \text{int list list}$ ,  $\text{flatten } LL \cong \text{oldFlat } LL$ .

## mapping and combinator examples:

```

(* tmap : ('a -> 'b) -> 'a tree -> 'b tree *)
fun tmap f Empty = Empty
  | tmap f (Node(l, x, r)) = Node(tmap f l, f x, tmap f r)
(* tfold: ('b * 'a * 'b -> 'b) -> 'b -> 'a tree -> 'b *)
fun tfold f z Empty = z
  | tfold f z Node(l,x,r) = f (tfold f z l, x, tfold f z r)
val stringify : int tree -> string tree = tmap Int.toString
val treesum = tfold (fn(a, x, b) => a + x + b) 0

```

```

fun mapEnum (f : int * 'a -> 'b) (L : 'a list) =
  let
    val comb_fn = fn (x, (i, L')) => (i + 1, f(i, x) :: L')
    val (_, result) = foldl comb_fn (0, []) L
  in
    foldl (op ::) [] result
  end

```

```

scanl f z [x1, x2, ..., xn] ==>
[z, f(x1, z), f(x2, f(x1, z))...f(xn, ..., f(x2, f(x1, n)))...]
fun scanl f z L =
  let
    fun comb (x, (fxz, L)) = (f (x, fxz), f (x, fxz) :: L)
    val (_, res) = foldl comb (z, [z]) L
  in
    foldl (op ::) [] res
  end
fun scanlCPS f z [] k = k ([], z)
  | scanlCPS f z (x :: xs) k = f (x, z)
    (fn z' => scanlCPS f z' xs
    (fn (L', x') => k (z :: L', x'))))

```

using recursion	using HOFs
<pre> fun ptn p [] = ([], [])     ptn p (x :: xs) =     let       val (R1, R2) = ptn p xs     in       if (p x) then         (x :: R1, R2) else         (R1, x :: R2) end </pre>	<pre> fun partition' p L =   foldr (fn (x, (R1, R2))     =&gt; if (p x) then       (x :: R1, R2) else       (R1, x :: R2))     ([], []) L </pre>

```

fun leaves Nub = []
  | leaves (Branch (L, C, R, v)) =
    (case (leaves L, leaves C, leaves R) of
      ([], [], []) => [v]
      | (resL, resC, resR) => (resL @ resC) @ resR)

```

Let  $n$  be the number of Branches in the tree.

- $W_{\text{leaves}}(0) = k_0$ ,  $W_{\text{leaves}}(1) = k_1$
- $W_{\text{leaves}}(n) = W_{\text{leaves}}(n_l) + W_{\text{leaves}}(n_c) + W_{\text{leaves}}(n_r) + W_{\text{@}}(n_l) + W_{\text{@}}(n_l + n_c) + k_2 = 3W_{\text{leaves}}\left(\frac{n}{3}\right) + kn$

There are  $\log_3 n$  levels, the work/node at level  $i$  is  $\frac{kn}{3^i}$ .

There are  $3^i$  nodes at level  $i$ .

$$\sum_{i=0}^{\log_3 n} 3^i \cdot \frac{kn}{3^i} = kn \log_3 n \Rightarrow W_{\text{leaves}}(n) \in O(n \log n)$$

- $S_{\text{leaves}}(n) = \max(S_{\text{leaves}}(n_l), S_{\text{leaves}}(n_c), S_{\text{leaves}}(n_r)) + \max(S_{\text{@}}(n_l), S_{\text{@}}(n_l + n_c)) + k_2 = S_{\text{leaves}}\left(\frac{n}{3}\right) + kn$

There are  $\log_3 n$  levels, the work/node at level  $i$  is  $\frac{kn}{3^i}$ .

There is 1 node at level  $i$ .

$$\sum_{i=0}^{\log_3 n} \frac{kn}{3^i} \leq \sum_{i=0}^{\infty} \frac{kn}{3^i} = \frac{kn}{1 - \frac{1}{3}} = \frac{3kn}{2} \Rightarrow S_{\text{leaves}}(n) \in O(n)$$